Removed filter options

SMTParser/issues.lean
@@ -20,7 +20,6 @@ set_option trace.auto.smt.stderr true
 
 set_option trace.querySMT.debug true
 set_option duper.throwPortfolioErrors false
-set_option querySMT.filterOpt 3
 
 set_option duper.collectDatatypes true
 
@@ -86,14 +85,54 @@ example (t : Type) (x : myType2 t) : ∃ y : t, x = const3 y ∨ x = const4 y :=
   duper
 
 example (t : Type) (x : myType2 t) : ∃ y : t, x = const3 y ∨ x = const4 y := by
-  querySMT
+  sorry -- querySMT
 
 -------------------------------------------------------------------------------------------
--- The example previously worked but now results in a deterministic timeout, figure out why (not sure which
--- commit caused this to stop working unfortunately)
+-- Bug in lean-auto's monomorphization procedure that causes preprocessing to fail for myProd
 
+structure myStructure where
+  field1 : Int
+  field2 : Int
+
+open myStructure
+
+-- This example works because `myStructure` is actually a structure (and hence has projections, meaning
+-- it does not require handmade selector functions)
+example (sum : myStructure → Int)
+  (hSum : ∀ x : Int, ∀ y : Int, sum (mk x y) = x + y)
+  (x : myStructure) : ∃ y : myStructure, sum y > sum x := by
+  querySMT
+
+inductive myProd (t1 t2 : Type _)
+| mk : t1 → t2 → myProd t1 t2
+
+open myProd
+
+-- This example can be processing without the have statement, but with the have statement, we get
+-- an error from lean-auto
+example (sum : myProd Int Int → Int)
+  (hSum : ∀ x : Int, ∀ y : Int, sum (mk x y) = x + y)
+  (x : myProd Int Int) : ∃ y : myProd Int Int, sum x < sum y := by
+  let _mk_sel0 : myProd ℤ ℤ → ℤ := myProd.rec (motive := fun _ => ℤ) fun arg0 arg1 => arg0
+  let _mk_sel1 : myProd ℤ ℤ → ℤ := myProd.rec (motive := fun _ => ℤ) fun arg0 arg1 => arg1
+  have test : _mk_sel0 x = 0 := sorry -- This triggers `unfoldProj :: myProd is not a structure`
+  duper [*] {portfolioInstance := 1}
+  -- When I fix this issue, send a PR or issue to lean-auto main since this is something that should be fixed in main too
+
+set_option maxHeartbeats 400000 in
+set_option trace.duper.timeout.debug true in
+set_option duper.throwPortfolioErrors true in
+example (sum : myProd Int Int → Int)
+  (hSum : ∀ x : Int, ∀ y : Int, sum (mk x y) = x + y)
+  (x : myProd Int Int) : ∃ y : myProd Int Int, sum x < sum y := by
+  sorry -- querySMT -- unfoldProj :: myProd is not a structure
+
+-------------------------------------------------------------------------------------------
+-- The example works only when duper.collectDatatypes is disabled
+
+set_option duper.collectDatatypes false in
 example (x y z a b : Int) : (x < y → y < z → x < z) ∧ (a < b ∨ b ≤ a) := by
-  sorry -- querySMT
+  querySMT
 
 -------------------------------------------------------------------------------------------
 -- cvc5 yields lemmas containing approximate (`?`) types
@@ -110,3 +149,7 @@ example (x y : Real) : x < y ∨ y ≤ x := by
 example (x y z : Nat) : x < y → y < z → x < z := by
   querySMT -- TODO: Look into incorporating `zify` in the preprocessing (or a better version of it)
 -/
+
+-- **TODO** Investigate whether `a < b` and `b > a` are equally usable
+-- for querySMT (there might be a world where GT appears in the problem but lean-auto
+-- and/or cvc5 normalize it to LT, resulting in an issue)
