SMTParser/QuerySMT.lean
@@ -9,42 +9,6 @@ initialize Lean.registerTraceClass `querySMT.debug
 
 namespace QuerySMT
 
-inductive filterOptTy where
-| noFilter
-| tautoFilter
-| duperFilter
-| duperCore
-deriving Inhabited
-
-open filterOptTy DataValue
-
-def filterOptToDataValue : filterOptTy → DataValue
-  | noFilter => ofNat 0
-  | tautoFilter => ofNat 1
-  | duperFilter => ofNat 2
-  | duperCore => ofNat 3
-
-def dataValueToFilterOpt : DataValue → Option filterOptTy
-  | ofNat 0 => some noFilter
-  | ofNat 1 => some tautoFilter
-  | ofNat 2 => some duperFilter
-  | ofNat 3 => some duperCore
-  | _ => none
-
-instance : KVMap.Value filterOptTy := ⟨filterOptToDataValue, dataValueToFilterOpt⟩
-
-register_option querySMT.filterOpt : filterOptTy := {
-  defValue := noFilter
-  descr := ""
-}
-
-def querySMT.getFilterOpt (opts : Options) : filterOptTy :=
-  querySMT.filterOpt.get opts
-
-def querySMT.getFilterOptM : CoreM filterOptTy := do
-  let opts ← getOptions
-  return querySMT.getFilterOpt opts
-
 /-- Checks whether the expression `e` can already be proven by `duper` -/
 def uselessLemma (e : Expr) : TacticM Bool := do
   withoutModifyingState do
@@ -105,45 +69,90 @@ def getNegGoalLemmaNameFromConfigOptions (configOptionsStx : TSyntaxArray `Query
 macro_rules
 | `(tactic| querySMT) => `(tactic| querySMT {})
 
-/-- Given `smtLemmas` output by the SMT solver and `lemmas` which is output by `Auto.collectAllLemmas`,
-    `getDuperCoreSMTLemmas` calls Duper and returns just the SMT lemmas that appear in the final proof -/
-def getDuperCoreSMTLemmas (smtLemmas : List Expr) (lemmas : Array Auto.Lemma) : TacticM (List Expr) := do
-  -- Preprocess `smtLemmas` to zetaReduce let expressions
-  -- Note: We don't need to preprocess `lemmas` because `Auto.collectAllLemmas` already zetaReduces
-  let smtLemmas ← smtLemmas.mapM (fun lem => Duper.preprocessFact lem)
-  let smtDeclInfos : Array (Name × (Array Expr → TacticM Expr)) := Id.run do
-    let mut declInfos := #[]
-    let mut declCounter := 0
-    let baseName := `h
-    for lem in smtLemmas do
-      let lemName := Name.num baseName declCounter
-      let lemConstructor : Array Expr → TacticM Expr := (fun _ => pure lem)
-      declInfos := declInfos.push (lemName, lemConstructor)
-      declCounter := declCounter + 1
-    pure declInfos
-  withLocalDeclsD smtDeclInfos $ fun xs => do
-    let formulas ← do
-      let mut formulas := #[]
-      let mut lemCounter := 0
-      for lem in smtLemmas do -- Add SMT lemmas
-        formulas := formulas.push (lem, ← mkAppM ``eq_true #[xs[lemCounter]!], #[], false)
-        lemCounter := lemCounter + 1
-      for lem in lemmas do -- Add lemmas from ordinary lctx (including the negated goal)
-        let isFromGoal := false -- **TODO**: Figure out how to correctly compute this using `goalDecls`
-        formulas := formulas.push (lem.type, ← mkAppM ``eq_true #[lem.proof], lem.params, isFromGoal)
-      pure formulas.toList
-    let duperConfigOptions :=
-      { portfolioMode := true, portfolioInstance := none, inhabitationReasoning := none,
-        preprocessing := none, includeExpensiveRules := none, selFunction := none }
-    let prf ← runDuperPortfolioMode formulas none duperConfigOptions none
-    let mut smtLemmasInPrf := #[]
-    let mut smtDeclIndex := 0
-    for x in xs do
-      if prf.containsFVar x.fvarId! then
-        trace[querySMT.debug] "{smtLemmas[smtDeclIndex]!} appears in the proof (index: {smtDeclIndex})"
-        smtLemmasInPrf := smtLemmasInPrf.push (smtLemmas[smtDeclIndex]!)
-      smtDeclIndex := smtDeclIndex + 1
-    pure smtLemmasInPrf.toList
+/-- Given `selectorInfos` and `smtLemmas` output by the SMT solver, and `lemmas` which is output by
+    `Auto.collectAllLemmas`, `getDuperCoreSMTLemmas` calls Duper and returns:
+    - The selectorInfos corresponding to selectors that appear in the final proof
+    - The SMT lemmas that appear in the final proof -/
+def getDuperCoreSMTLemmas (selectorInfos : Array (String × Expr × Nat × Expr)) (smtLemmas : List Expr)
+  (lemmas : Array Auto.Lemma) : TacticM (List Expr) := do
+  /- **TODO** Incorporate `selectorInfos`
+  -- Add selectors to the local context and instantiate `smtLemmas` with them
+  for (selName, selCtor, argIdx, selType) in selectorInfos do
+    let selTypeStx ← withOptions (fun o => (o.set `pp.analyze true).set `pp.proofs true) $ PrettyPrinter.delab selType
+    let selector ← buildSelector selCtor argIdx
+    let selectorStx ← withOptions (fun o => (o.set `pp.analyze true).set `pp.proofs true) $ PrettyPrinter.delab selector
+    evalTactic $ ← `(tactic| let $(mkIdent (.str .anonymous selName)) : $selTypeStx := $selectorStx) -- Add selector to lctx
+  -/
+  withMainContext do -- Use updated main context so that newly added selectors are accessible
+    /- **TODO** Incorporate `selectorInfos`
+    let lctx ← getLCtx
+    let mut selectorFVars := #[]
+    for (selUserName, _, _, _) in selectorInfos do
+      match lctx.findFromUserName? (.str .anonymous selUserName) with
+      | some decl => selectorFVars := selectorFVars.push (.fvar decl.fvarId)
+      | none => throwError "getDuperCoreSMTLemmas :: Error in trying to access selector definition for {selUserName}"
+    let smtLemmas := smtLemmas.map (fun lem => lem.instantiateRev selectorFVars)
+    -/
+    /- Preprocess `smtLemmas` to zetaReduce let expressions
+      We don't need to preprocess `lemmas` because `Auto.collectAllLemmas` already zetaReduces -/
+    let smtLemmas ← smtLemmas.mapM (fun lem => Duper.preprocessFact lem)
+    let smtDeclInfos : Array (Name × (Array Expr → TacticM Expr)) ← do
+      let mut declInfos := #[]
+      let mut declCounter := 0
+      let baseName := `h
+      for lem in smtLemmas do
+        let lemName := Name.num baseName declCounter
+        let lemConstructor : Array Expr → TacticM Expr := (fun _ => pure lem)
+        declInfos := declInfos.push (lemName, lemConstructor)
+        declCounter := declCounter + 1
+      pure declInfos
+    withLocalDeclsD smtDeclInfos $ fun xs => do
+      let formulas ← do
+        let mut formulas := #[]
+        let mut lemCounter := 0
+        for lem in smtLemmas do -- Add SMT lemmas
+          formulas := formulas.push (lem, ← mkAppM ``eq_true #[xs[lemCounter]!], #[], false)
+          lemCounter := lemCounter + 1
+        for lem in lemmas do -- Add lemmas from ordinary lctx (including the negated goal)
+          let isFromGoal := false -- **TODO**: Figure out how to correctly compute this using `goalDecls`
+          formulas := formulas.push (lem.type, ← mkAppM ``eq_true #[lem.proof], lem.params, isFromGoal)
+        /- **TODO** Incorporate `selectorInfos`
+        for ((selName, selCtor, argIdx, selType), selectorFVar) in selectorInfos.zip selectorFVars do
+          /- Add Duper-friendly facts about the selectors (Each selector corresponding to argument `i`
+            of constructor `c` returns the `i`th argument of `c` when given `c`) -/
+          let selCtorType ← inferType selCtor
+          let selCtorFieldTypes := getForallArgumentTypes selCtorType
+          let selCtorDeclInfos : Array (Name × (Array Expr → TacticM Expr)) ← do
+            let mut declInfos := #[]
+            let mut declCounter := 0
+            let baseName := `arg
+            for selCtorFieldType in selCtorFieldTypes do
+              let argName := Name.num baseName declCounter
+              let argConstructor : Array Expr → TacticM Expr := (fun _ => pure selCtorFieldType)
+              declInfos := declInfos.push (argName, argConstructor)
+              declCounter := declCounter + 1
+            pure declInfos
+          let selectorHyp ←
+            withLocalDeclsD selCtorDeclInfos $ fun selCtorArgFVars => do
+              let selCtorWithFields ← mkAppM' selCtor selCtorArgFVars
+              let selectedArg := selCtorArgFVars[argIdx]!
+              mkForallFVars selCtorArgFVars $ ← mkAppM ``Eq #[← mkAppM' selectorFVar #[selCtorWithFields], selectedArg]
+          trace[querySMT.debug] "Adding selectorHyp: {selectorHyp} to formulas"
+          formulas := formulas.push (selectorHyp, ← mkSorry (← mkAppM ``Eq #[selectorHyp, mkConst ``True]) false, #[], false)
+        -/
+        pure formulas.toList
+      let duperConfigOptions :=
+        { portfolioMode := true, portfolioInstance := none, inhabitationReasoning := none,
+          preprocessing := none, includeExpensiveRules := none, selFunction := none }
+      let prf ← runDuperPortfolioMode formulas none duperConfigOptions none
+      let mut smtLemmasInPrf := #[]
+      let mut smtDeclIndex := 0
+      for x in xs do
+        if prf.containsFVar x.fvarId! then
+          trace[querySMT.debug] "{smtLemmas[smtDeclIndex]!} appears in the proof (index: {smtDeclIndex})"
+          smtLemmasInPrf := smtLemmasInPrf.push (smtLemmas[smtDeclIndex]!)
+        smtDeclIndex := smtDeclIndex + 1
+      pure smtLemmasInPrf.toList
 
 /-- Copied from Lean.Meta.Tactic.Intro.lean -/
 private partial def getIntrosSize : Expr → Nat
@@ -167,7 +176,7 @@ def evalQuerySMT : Tactic
   let numBinders := getIntrosSize goalType
   let (goalBinders, newGoal) ← introNCore originalMainGoal numBinders [] true true
   let [nngoal] ← newGoal.apply (.const ``Classical.byContradiction [])
-    | throwError "evalAuto :: Unexpected result after applying Classical.byContradiction"
+    | throwError "querySMT :: Unexpected result after applying Classical.byContradiction"
   let (_, absurd) ← MVarId.intro1 nngoal
   replaceMainGoal [absurd]
   withMainContext do
@@ -179,23 +188,18 @@ def evalQuerySMT : Tactic
     | some skolemPrefix => evalTactic (← `(tactic| skolemizeAll {prefix := $(Syntax.mkStrLit skolemPrefix)}))
     | none => evalTactic (← `(tactic| skolemizeAll))
     let goalsAfterSkolemization ← getGoals
-    let newAbsurd ← getMainGoal
     withMainContext do -- Testing whether this fixes things
       let (lemmas, inhFacts) ← collectAllLemmas (← `(hints| [*])) uords #[]
       let allSMTLemmas ← runAutoGetHints lemmas inhFacts
-      let (preprocessFacts, theoryLemmas, instantiations, rewriteFacts) := allSMTLemmas
+      let (selectorInfos, preprocessFacts, theoryLemmas, instantiations, rewriteFacts) := allSMTLemmas
       let smtLemmas := preprocessFacts ++ theoryLemmas ++ -- instantiations
         (rewriteFacts.foldl (fun acc rwFacts => acc ++ rwFacts) [])
       trace[querySMT.debug] "Number of lemmas before filter: {smtLemmas.length}"
-      let smtLemmas ←
-        match ← querySMT.getFilterOptM with
-        | noFilter => pure smtLemmas
-        | tautoFilter => smtLemmas.filterM (fun lem => return !(← isTautology lem))
-        | duperFilter => smtLemmas.filterM (fun lem => return !(← uselessLemma lem))
-        | duperCore => getDuperCoreSMTLemmas smtLemmas lemmas
+      let smtLemmas ← getDuperCoreSMTLemmas selectorInfos smtLemmas lemmas
       trace[querySMT.debug] "Number of lemmas after filter: {smtLemmas.length}"
+      -- **TODO** Also need to make syntax for creating selectors and their corresponding facts
       let lemmasStx ← smtLemmas.mapM
-        (fun lemExp => withOptions (fun o => o.set `pp.analyze true) $ PrettyPrinter.delab lemExp)
+        (fun lemExp => withOptions (fun o => (o.set `pp.analyze true).set `pp.proofs true) $ PrettyPrinter.delab lemExp)
       let mut tacticsArr := #[] -- The array of tactics that will be suggested to the user
       -- Build the `intros ...` tactic with appropriate names
       let mut introsNames : Array Name := #[]
@@ -242,6 +246,7 @@ def evalQuerySMT : Tactic
       -- Create the suggestion
       addTryThisTacticSeqSuggestion stxRef tacticSeq (← getRef)
       let proof ← mkAppM ``sorryAx #[Expr.const ``False [], Expr.const ``false []]
+      let newAbsurd ← getMainGoal -- Main goal changed by `skolemizeAll` and selector creation
       newAbsurd.assign proof
 | _ => throwUnsupportedSyntax
 
